Finish main part of compute_nested_efield_spec. Some progress in more integrated loadstore rules.

floyd/efield_lemmas.v
@@ -26,13 +26,6 @@ Fixpoint nested_efield (e: expr) (efs: list efield) (tts: list type) : expr :=
     end
   end.
 
-Definition compute_lr e (efs: list efield) :=
-  match typeof e, length efs with
-  | Tpointer _ _, S _ => RRRR
-  | Tarray _ _ _, _ => RRRR (* This line can be either L or R, but R is consistent with LR_of_type *)
-  | _, _ => LLLL
-  end.
-
 Inductive array_subsc_denote {cs: compspecs}: expr -> Z -> environ -> Prop :=
   | array_subsc_denote_intro:
       forall e i rho, Vint (Int.repr i) = eval_expr e rho -> array_subsc_denote e i rho.
@@ -193,8 +186,8 @@ Proof.
 Qed.
 
 Definition LR_of_type (t: type) :=
-  match access_mode t with
-  | By_reference => RRRR
+  match t with
+  | Tarray _ _ _ => RRRR
   | _ => LLLL
   end.
 
@@ -487,11 +480,12 @@ Proof.
     apply andp_left2.
     unfold LR_of_type in H2.
     subst.
-    destruct (access_mode (typeof e)) eqn:?H; inv H2.
+    destruct (typeof e) eqn:?H; inv H2.
     apply andp_right.
     - eapply derives_trans; [apply By_reference_eval_expr |]; auto.
-      normalize.
+      rewrite H; auto. normalize.
     - apply By_reference_tc_expr; auto.
+      rewrite H; auto.
 Qed.
 
 Lemma eval_lvalue_nested_efield_aux: forall Delta t_root e efs gfs tts p,
@@ -586,77 +580,173 @@ Proof.
   destruct (nested_field_type t_root gfs) as [| [| | |] [|] | | [|] | | | | |]; inv H2; inv H0.
 Qed.
 
-Definition compute_nested_efield {cs: compspecs}: expr -> expr * list efield * list type * LLRR :=
-  fix compute_nested_efield e :=
+Fixpoint compute_nested_efield_rec {cs:compspecs} e lr_default :=
   match e with
   | Efield e' id t =>
     match typeof e' with
     | Tstruct id_str _ =>
       if eqb_type (field_type id (co_members (get_co id_str))) t
-      then match compute_nested_efield e' with
+      then match compute_nested_efield_rec e' LLLL with
            | (e'', efs, tts, lr) => (e'', eStructField id :: efs, t :: tts, lr)
            end
-      else (e, nil, nil, LLLL)
+      else (e, nil, nil, lr_default)
     | Tunion id_uni _ =>
       if eqb_type (field_type id (co_members (get_co id_uni))) t
-      then match compute_nested_efield e' with
+      then match compute_nested_efield_rec e' LLLL with
            | (e'', efs, tts, lr) => (e'', eUnionField id :: efs, t :: tts, lr)
            end
-      else (e, nil, nil, LLLL)
-    | _ => (e, nil, nil, LLLL)
+      else (e, nil, nil, lr_default)
+    | _ => (e, nil, nil, lr_default)
     end
   | Ederef (Ebinop Oadd e' ei (Tpointer t a)) t' =>
-    match typeof e', eqb_type t t', eqb_attr a noattr with
-    | Tarray _ _ _, true, true =>
-      match compute_nested_efield e' with
-      | (e'', efs, tts, lr) => (e'', eArraySubsc ei :: efs, t :: tts, lr)
+    match typeof e' with
+    | Tarray t'' _ _ =>
+      match eqb_type t t'', eqb_type t t', eqb_attr a noattr with
+      | true, true, true =>
+        match compute_nested_efield_rec e' RRRR with
+        | (e'', efs, tts, lr) => (e'', eArraySubsc ei :: efs, t :: tts, lr)
+        end
+      | _, _, _ => (e, nil, nil, lr_default)
       end
-    | Tpointer _ _, true, true => (e', eArraySubsc ei :: nil, t :: nil, RRRR)
-    | _, _, _ => (e, nil, nil, LLLL)
+    | Tpointer t'' _ =>
+      match eqb_type t t'', eqb_type t t', eqb_attr a noattr with
+      | true, true, true => (e', eArraySubsc ei :: nil, t :: nil, RRRR)
+      | _, _, _ => (e, nil, nil, lr_default)
+      end
+    | _ => (e, nil, nil, lr_default)
     end
-  | _ => (e, nil, nil, LLLL)
+  | _ => (e, nil, nil, lr_default)
   end.
+
+Definition compute_nested_efield {cs: compspecs} (e: expr): expr * list efield * list type * LLRR := compute_nested_efield_rec e LLLL.
 
 Inductive compute_root_type: forall (t_from_e: type) (lr: LLRR) (t_root: type), Prop :=
   | compute_root_type_lvalue: forall t, compute_root_type t LLLL t
   | compute_root_type_expr: forall t a1 n a2, compute_root_type (Tpointer t a1) RRRR (Tarray t n a2).
 
-Lemma compute_nested_efield_aux: forall e t,
-  match compute_nested_efield e with
-  | (e', gfs, tts, lr) => nested_efield e' gfs tts = e
-  end /\
-  match compute_nested_efield (Ederef e t) with
-  | (e', gfs, tts, lr) => nested_efield e' gfs tts = Ederef e t
+(* which means (e, lr) is possible to be called by compute_nested_efield_rec *)
+Definition LR_possible (e: expr) (lr: LLRR) : bool :=
+  match lr with
+  | LLLL => match (typeof e) with
+                              | Tarray _ _ _ => false
+                              | _ => true
+            end
+  | RRRR => match (typeof e) with
+            | Tarray _ _ _ => true
+            | _ => false
+            end
   end.
+
+Lemma compute_nested_efield_trivial: forall e rho lr_default,
+  forall e_root efs tts lr,
+  e_root = e -> efs = nil -> tts = nil -> lr = lr_default ->
+  LR_possible e lr_default = true ->
+    forall t_root gfs,
+      compute_root_type (typeof e_root) lr t_root ->
+      efield_denote efs gfs rho ->
+      nested_efield e_root efs tts = e /\
+      LR_of_type t_root = lr /\
+      legal_nested_efield_rec t_root gfs tts = true /\
+      nested_field_type t_root gfs = typeof e.
 Proof.
   intros.
-  revert t.
-  induction e; intros; split; try reflexivity.
-  + destruct (IHe t).
-    exact H0.
-  + clear IHe2.
-    destruct (IHe1 t) as [? _]; clear IHe1.
-    simpl; destruct b, t; try reflexivity.
-    destruct (compute_nested_efield e1) as (((?, ?), ?), ?); try reflexivity.
-    destruct (typeof e1); try reflexivity.
-    - destruct (eqb_type t t0) eqn:?H; try reflexivity.
-      apply eqb_type_spec in H0.
-      destruct (eqb_attr a noattr) eqn:?H; try reflexivity.
-      apply eqb_attr_spec in H1.
-      subst.
-      reflexivity.
-    - destruct (eqb_type t t0) eqn:?H; try reflexivity.
-      apply eqb_type_spec in H0.
-      destruct (eqb_attr a noattr) eqn:?H; try reflexivity.
-      apply eqb_attr_spec in H1.
-      subst.
-      reflexivity.
-  + destruct (IHe t) as [? _]; clear IHe.
+  subst.
+  unfold LR_possible in H3.
+  destruct (typeof e); inv H3; inv H4; inv H5; cbv; auto.
+  + inv H0.
+  + destruct e; inv H0.
+Qed.
+
+Lemma compute_nested_efield_aux: forall e rho lr_default,
+  (LR_possible e lr_default = true ->
+  match compute_nested_efield_rec e lr_default with
+  | (e_root, efs, tts, lr) =>
+    forall t_root gfs,
+      compute_root_type (typeof e_root) lr t_root ->
+      efield_denote efs gfs rho ->
+      nested_efield e_root efs tts = e /\
+      LR_of_type t_root = lr /\
+      legal_nested_efield_rec t_root gfs tts = true /\
+      nested_field_type t_root gfs = typeof e
+  end) /\
+  forall t,
+  (LR_possible (Ederef e t) lr_default = true ->
+  match compute_nested_efield_rec (Ederef e t) lr_default with
+  | (e_root, efs, tts, lr) =>
+      forall t_root gfs,
+      compute_root_type (typeof e_root) lr t_root ->
+      efield_denote efs gfs rho ->
+      nested_efield e_root efs tts = Ederef e t /\
+      LR_of_type t_root = lr /\
+      legal_nested_efield_rec t_root gfs tts = true /\
+      nested_field_type t_root gfs = typeof (Ederef e t)
+  end).
+Proof.
+  intros ? ?.
+  induction e; intros ?; (split; [ | intros ?]);
+  try exact (compute_nested_efield_trivial _ _ _ _ _ _ _ eq_refl eq_refl eq_refl eq_refl).
+  + destruct (IHe lr_default). apply (H0 t).
+  + destruct b, t; try exact (compute_nested_efield_trivial _ _ _ _ _ _ _ eq_refl eq_refl eq_refl eq_refl).
     simpl.
-    destruct (compute_nested_efield e) as (((?, ?), ?), ?); try reflexivity.
-    destruct (typeof e); try reflexivity.
-    - if_tac; auto. simpl. rewrite <- H. reflexivity.
-    - if_tac; auto. simpl. rewrite <- H. reflexivity.
+    destruct (typeof e1) eqn:?H; try exact (compute_nested_efield_trivial _ _ _ _ _ _ _ eq_refl eq_refl eq_refl eq_refl);
+    destruct (eqb_type t t1) eqn:?H; try exact (compute_nested_efield_trivial _ _ _ _ _ _ _ eq_refl eq_refl eq_refl eq_refl);
+    apply eqb_type_spec in H0;
+    destruct (eqb_type t t0) eqn:?H; try exact (compute_nested_efield_trivial _ _ _ _ _ _ _ eq_refl eq_refl eq_refl eq_refl);
+    apply eqb_type_spec in H1;
+    destruct (eqb_attr a noattr) eqn:?H; try exact (compute_nested_efield_trivial _ _ _ _ _ _ _ eq_refl eq_refl eq_refl eq_refl);
+    apply eqb_attr_spec in H2.
+    - subst.
+      intros.
+      inv H1; inv H2.
+      inv H9.
+      rewrite H in H4; inv H4.
+      simpl.
+      change (nested_field_type (Tarray t0 n a2) (SUB i)) with t0.
+      rewrite eqb_type_spec.
+      auto.
+    - subst.
+      destruct (IHe1 RRRR) as [IH _]; spec IH; [unfold LR_possible; rewrite H; auto |].
+      clear IHe1 IHe2.
+      destruct (compute_nested_efield_rec e1 RRRR) as (((?, ?), ?), ?).
+      intros.
+      inv H2.
+      specialize (IH _ _ H1 H9).
+      destruct IH as [IH1 [IH2 [IH3 IH4]]].
+      simpl.
+      rewrite IH1, IH3, nested_field_type_ind, IH4.
+      simpl.
+      rewrite eqb_type_spec.
+      auto.
+  + Opaque field_type. simpl. Transparent field_type.
+    destruct (typeof e) eqn:?H; try exact (compute_nested_efield_trivial _ _ _ _ _ _ _ eq_refl eq_refl eq_refl eq_refl);
+    destruct (eqb_type (field_type i (co_members (get_co i0))) t) eqn:?H; try exact (compute_nested_efield_trivial _ _ _ _ _ _ _ eq_refl eq_refl eq_refl eq_refl);
+    apply eqb_type_spec in H0.
+    - intros.
+      destruct (IHe LLLL) as [IH _]; clear IHe.
+      spec IH; [unfold LR_possible; rewrite H; auto |].
+      destruct (compute_nested_efield_rec e LLLL) as (((?, ?), ?), ?).
+      intros.
+      revert H0; inv H3; intros.
+      specialize (IH _ _ H2 H7).
+      destruct IH as [IH1 [IH2 [IH3 IH4]]].
+      simpl.
+      rewrite IH1, IH3, nested_field_type_ind, IH4.
+      simpl.
+      rewrite eqb_type_spec.
+      auto.
+    - intros.
+      destruct (IHe LLLL) as [IH _]; clear IHe.
+      spec IH; [unfold LR_possible; rewrite H; auto |].
+      destruct (compute_nested_efield_rec e LLLL) as (((?, ?), ?), ?).
+      intros.
+      revert H0; inv H3; intros.
+      specialize (IH _ _ H2 H7).
+      destruct IH as [IH1 [IH2 [IH3 IH4]]].
+      simpl.
+      rewrite IH1, IH3, nested_field_type_ind, IH4.
+      simpl.
+      rewrite eqb_type_spec.
+      auto.
 Qed.
 
 Lemma compute_nested_efield_lemma: forall e,
